refactor into multiple files

coq/denot.v
@@ -1,554 +1,370 @@
-Require Export lc.tactics.
-Require Export lc.relations.
-Require Import Lia.
 Require Import Coq.Logic.FunctionalExtensionality.
+Require Import Coq.Classes.RelationClasses.
+Require Coq.Relations.Relation_Definitions.
+Require Import Lia.
 
+Require Export lc.tactics.
+
+Require Import lc.List.
+Require Import lc.Env.
+
+Require Import lc.SetsAsPredicates.
+Import SetNotations.
+Local Open Scope set_scope.
+
+Require Import lc.Monad.
+Import MonadNotation.
+Open Scope monad_scope.
+
+Require Import lc.Container.
+
+Require Import lc.Scoped.
+
+Require Import lc.model_definitions.
+
+Import EnvNotations.
 Import LCNotations.
-Local Open Scope lc_scope.
+
+Import Wf_nat.
+
+(* This cannot be part of the Env module because we need to know the type
+   of the domain *)
+Ltac gather_atoms ::=
+  let A := gather_atoms_with (fun x : vars => x) in
+  let B := gather_atoms_with (fun x : var => {{ x }}) in
+  let C := gather_atoms_with (fun x => fv_tm x) in
+  let D := gather_atoms_with (fun x : list (atom * P Value) => dom x) in
+  constr:(A \u B \u C \u D).
 
 
-(* This is a Coq port of https://plfa.github.io/Denotational/ *)
-(* It is a filter model of the lambda calculus *)
-
-(* What changes if we want to do CBV instead? *)
-(* What if we want to add "WRONG", i.e. for unbound variables? *)
-(* What if we want to add other values (i.e. nats, lists, etc)? *)
-
-Inductive Value : Type :=
-  | v_bot   : Value
-  | v_map   : Value -> Value -> Value
-  | v_union : Value -> Value -> Value
-.
-
-Notation "⊥" := v_bot.
-Infix "↦" := v_map (at level 90, right associativity).
-Infix "⊔" := v_union (at level 85, right associativity).
-
-(* Approximate values *)
-
-Reserved Notation "v1 ⊑ v2" (at level 55).
-Inductive v_sub : Value -> Value -> Prop :=
-  | v_sub_bot : forall v, ⊥ ⊑ v
-  | v_sub_conj_L : forall u v w, 
-      (v ⊑ u) -> (w ⊑ u) -> ((v ⊔ w) ⊑ u)
-  | v_sub_conj_R1 : forall u v w, 
-      u ⊑ v -> u ⊑ (v ⊔ w)      
-  | v_sub_conj_R2 : forall u v w, 
-      u ⊑ w -> u ⊑ (v ⊔ w)
-  | v_sub_trans : forall u v w, 
-      u ⊑ v -> v ⊑ w -> u ⊑ w
-  | v_sub_fun : forall v w v' w', 
-      v' ⊑ v
-      -> w ⊑ w'
-      -> (v ↦ w) ⊑ (v' ↦ w')
-  | v_sub_dist : forall v w w', 
-      (v ↦ (w ⊔ w')) ⊑ ((v ↦ w) ⊔ (v ↦ w'))
-where "v1 ⊑ v2" := (v_sub v1 v2).
-
-#[global] Hint Constructors v_sub : core.
-
-Lemma v_sub_refl : forall v, v ⊑ v.
+Lemma size_is_enough : forall n a, n >= size_tm a -> forall ρ, denot_n n a ρ = denot_n (size_tm a) a ρ.
 Proof.
-  intro v. induction v; eauto.
+  intros n.
+  induction (lt_wf n) as [n _ IH].
+  intros a h ρ; destruct a; simpl in *.
+  all: try destruct n; simpl; auto; try lia.
+  all: f_equal.
+  all: try rewrite IH; try lia; auto;
+    try rewrite IH; try lia; auto.
+  - extensionality D.
+    remember (fresh_for (dom ρ \u fv_tm a)) as x.
+    rewrite IH. lia.
+    autorewrite with lngen. lia.
+    autorewrite with lngen. auto.
+Qed.
+
+Definition denot (a : tm) := denot_n (size_tm a) a.
+
+Lemma denot_var_b : forall x ρ, denot (var_b x) ρ = ⌈ v_wrong ⌉.
+Proof.
+  intros x ρ. reflexivity.
+Qed.
+
+Lemma denot_var : forall x ρ, denot (var_f x) ρ = ρ ⋅ x.
+Proof.
+  intros. reflexivity.
+Qed.
+
+Lemma denot_app : forall t u ρ, 
+    denot (app t u) ρ = 
+      (denot t ρ ▩ denot u ρ).
+Proof. 
+  intros.
+  unfold denot. simpl.
+  rewrite size_is_enough. lia. auto.
+  rewrite size_is_enough. lia. auto.
+Qed.
+
+Lemma denot_lit : forall k ρ,  denot (lit k) ρ = NAT k.
+Proof. intros. reflexivity. Qed. 
+
+Lemma denot_add : forall ρ,  denot add ρ = ADD.
+Proof. intros. reflexivity. Qed. 
+
+Lemma denot_tnil : forall ρ,  denot tnil ρ = NIL.
+Proof.  intros. reflexivity. Qed. 
+
+Lemma denot_tcons : forall t u ρ, 
+    denot (tcons t u) ρ = CONS (denot t ρ) (denot u ρ).
+Proof. 
+  intros.
+  unfold denot. simpl.
+  rewrite size_is_enough. lia. auto.
+  rewrite size_is_enough. lia. auto.
+Qed.
+
+
+(* To compute the denotation of an abstraction, we need to first prove a
+   renaming lemma. This lemma ensures that the names that we pick for the
+   lambda-bound variables don't matter.  *)
+
+Ltac name_binder x0 Frx0 := 
+    match goal with 
+      [ |- context[fresh_for ?ρ] ] => 
+         remember (fresh_for ρ) as x0;
+         move: (@fresh_for_fresh x0 ρ ltac:(auto)) => Frx0;
+         simpl_env in Frx0
+    end.    
+
+Definition access_app_P := @access_app (P Value) ⌈ v_wrong ⌉.
+
+(* Renaming property for denotations. *)
+
+Lemma rename_denot_n : forall n t y w ρ1 ρ2 D, 
+  w `notin` dom ρ1 -> 
+  y `notin` dom ρ1 \u fv_tm t -> 
+  denot_n n t (ρ1 ++ w ~ D ++ ρ2) = 
+  denot_n n (t [w ~> var_f y]) (ρ1 ++ y ~ D ++ ρ2).
+Proof. 
+  induction n;
+  intros t y w ρ1 ρ2 D Frw Fry; simpl. auto.
+  destruct t; simpl; auto.
+  all: simpl in Fry.
+  + destruct (x == w).
+    ++ subst. 
+       simpl_env.       
+       rewrite access_app_fresh; auto. 
+       rewrite access_eq_var.
+       rewrite access_app_fresh; auto. 
+       rewrite access_eq_var. auto.
+    ++ have NEx: x <> y. fsetdec.
+       edestruct (@access_app_P ρ1 x).
+       repeat rewrite H. auto.
+       destruct (H (cons (w, D) ρ2)).
+       rewrite H1. 
+       destruct (H (cons (y, D) ρ2)).
+       rewrite H3.
+       rewrite access_neq_var. auto.
+       rewrite access_neq_var. auto.
+       auto.
+  + f_equal.
+    extensionality D0.
+    name_binder x0 Frx0.
+    name_binder y0 Fry0.
+
+    pick fresh z.
+    rewrite (subst_tm_intro z _ (var_f x0)). 
+    auto. 
+    rewrite (subst_tm_intro z _ (var_f y0)). 
+    { autorewrite with lngen. simpl.
+      clear Frx0 Fry0 Fry Frw. fsetdec. }
+    replace (t [w ~> var_f y] ^ z) with ((t ^ z) [w ~> var_f y]).
+    2: {
+      rewrite subst_tm_open_tm_wrt_tm; auto.
+      rewrite subst_neq_var. 
+      fsetdec.
+      auto.
+    } 
+    rewrite <- cons_app_assoc.
+
+    replace (((x0, D0) :: ρ1) ++ (w, D) :: ρ2) with
+      (nil ++ (x0 ~ D0) ++ (ρ1 ++ (w ~ D) ++ ρ2)). 2: { simpl_env; auto. }
+    rewrite <- IHn; simpl_env; auto.
+    2: { autorewrite with lngen. 
+         clear Fry0 Frw Fry.
+         simpl.
+         fsetdec.
+    }
+
+    replace ((y0 ~ D0) ++ ρ1 ++ (y ~ D) ++ ρ2) with
+      (nil ++ (y0 ~ D0) ++ (ρ1 ++ (y ~ D) ++ ρ2)). 2: { simpl_env; auto. }
+
+    rewrite <- IHn; simpl_env; auto.
+    2: { rewrite fv_tm_subst_tm_upper.            
+         rewrite fv_tm_open_tm_wrt_tm_upper.
+         simpl.
+         clear Frx0 Frw Fry.
+         rewrite <- fv_tm_subst_tm_lower in Fry0.
+         fsetdec.
+    }
+    
+    repeat rewrite <- (app_assoc _ (z ~ D0)).
+    eapply IHn.
+    simpl_env. { clear Fry0 Fry Frx0. fsetdec. }
+    rewrite fv_tm_open_tm_wrt_tm_upper.
+    simpl_env. simpl.
+
+    clear Frx0 Fry0 Frw.
+    simpl in Fry.
+    fsetdec.
+  + simpl_env.
+    f_equal.
+    apply IHn; simpl_env; auto.
+    apply IHn; simpl_env; auto.
+  + simpl_env.
+    f_equal.
+    apply IHn; simpl_env; auto.
+    apply IHn; simpl_env; auto. 
+Qed.
+
+
+Lemma rename_open_denot : forall w y n t  ρ D, 
+  w `notin` fv_tm t -> 
+  y `notin` fv_tm t -> 
+  denot_n n (t ^ w) (w ~ D ++ ρ) = 
+  denot_n n (t ^ y) (y ~ D ++ ρ).
+Proof. 
+  intros.
+  pick fresh z.
+  rewrite (subst_tm_intro z _ (var_f w)). auto.
+  rewrite (subst_tm_intro z _ (var_f y)). auto.
+  rewrite_env (nil ++ w ~ D ++ ρ).
+  rewrite <- rename_denot_n; simpl; auto.
+  rewrite_env (nil ++ y ~ D ++ ρ).
+  rewrite <- rename_denot_n; simpl; auto.
+  rewrite fv_tm_open_tm_wrt_tm_upper. simpl. fsetdec.
+  rewrite fv_tm_open_tm_wrt_tm_upper. simpl. fsetdec.
 Qed.  
 
-#[global] Hint Resolve v_sub_refl : core.
-
-#[global] Instance Refl_v_sub : Reflexive v_sub.
-unfold Reflexive. eauto. Qed.
-
-Lemma v_sub_mono : forall (v w v' w': Value), 
-    v ⊑ v' -> (w ⊑ w') ->
-    (v ⊔ w) ⊑ (v' ⊔ w').
-Proof. 
-  intros; eauto.
-Qed.
-
-(* ⊔↦⊔-dist *)
-Lemma v_sub_union_dist : forall (v w v' w': Value), 
-    (v ⊔ v' ↦ w ⊔ w') ⊑ ((v ↦ w) ⊔ (v' ↦ w')).
-Proof. intros. 
-       eapply v_sub_trans.
-       eapply v_sub_dist.
-       eapply v_sub_mono.
-       + eapply v_sub_fun; eauto.
-       + eauto.
-Qed.
-
-Lemma v_sub_union_invL : forall u v w,
-    (u ⊔ v) ⊑ w -> u ⊑ w.
-Proof. intros u v w H. dependent induction H; eauto. Qed.
-
-Lemma v_sub_union_invR : forall u v w,
-    (u ⊔ v) ⊑ w -> v ⊑ w.
-Proof. intros u v w H. dependent induction H; eauto. Qed.
-
-
-(* Environments are maps of variables to values. We don't 
-   index by the current scope to avoid dependently-typed 
-   programming in Coq. 
-*)
-
-Definition Env := atom -> Value.
-
-Definition empty : Env := fun x => v_bot.
-
-Definition cons : atom -> Value -> Env -> Env := 
-  fun x v γ => fun y => match (x == y) with 
-                  | left _ => v
-                  | right pf => γ y
-                  end.
-
-Definition env_sub (γ : Env) (δ : Env) : Prop :=
-  forall x, γ x ⊑ δ x.
-
-#[global] Instance Refl_env_sub : Reflexive env_sub.
-unfold Reflexive. intros γ. unfold env_sub. intros x. auto.
-Qed.
-
-#[global] Instance Trans_env_sub : Transitive env_sub.
-unfold Transitive. intros γ1 γ2 γ3. unfold env_sub. intros g1 g2 x. eauto.
-Qed.
-
-
-Lemma cons_cons : forall x y z v γ, 
-    z <> y ->
-    z <> x ->
-    cons y ((cons z v γ) x) (cons z v γ) = cons z v (cons y (γ x) γ).
+Lemma denot_abs : forall x t ρ,
+    x `notin` dom ρ \u fv_tm t ->
+    denot (abs t) ρ = 
+      Λ (fun D => denot (t ^ x) (x ~ D ++ ρ)).
 Proof.
   intros.
-  unfold cons.
-  extensionality w.
-  destruct (y == w) eqn:YW;
-  destruct (z == w) eqn:ZW; auto.
-  + subst. done. 
-  + subst. destruct (z == x). subst. done. done.
-Qed.     
-
-(* CBV requires that the value is not bot?? *)
-Inductive v_app : Value -> Value -> Value -> Prop :=
-  | app_beta : forall v w, 
-      (* CBV??      v <> v_bot -> *)
-      v_app (v ↦ w) v w
-.
-
-
-Inductive sem : Env -> tm -> Value -> Prop :=
-  | sem_var : forall γ x,
-      sem γ (var_f x) (γ x)
-  | sem_app : forall γ L M u v w,
-        sem γ L u
-      -> sem γ M v
-      -> v_app u v w
-      -> sem γ (app L M) w 
-  | sem_abs : forall L γ v w N,
-      (forall x, x `notin` L ->
-          sem (cons x v γ) (N ^ x) w) -> 
-      sem γ (abs N) (v ↦ w)
-  | bot_intro : forall γ M,
-      lc_tm M ->
-      sem γ M ⊥
-  | union_intro : forall γ M v w,
-      sem γ M v
-      -> sem γ M w
-      -> sem γ M (v ⊔ w)
-  | sem_sub : forall γ M v w,
-      sem γ M v
-      -> w ⊑ v
-      -> sem γ M w
-.
-
-#[global] Hint Constructors sem : core.
-
-Lemma sem_subst : forall x y γ M v,
-    y `notin` fv_tm M ->
-    sem γ M v ->
-    sem (cons y (γ x) γ) (subst_tm (var_f y) x M) v.
-Proof. 
-  intros.
-  induction H0.
-  all: simpl; simpl in H; eauto with lngen.
-  - have EQ: y <> x0. fsetdec.
-    destruct (x0 == x) eqn:E.
-    + subst. 
-      replace (γ x) with ((cons y (γ x) γ) y) at 2.
-      2: { unfold cons. destruct (y == y). auto. done. }
-      eapply sem_var. 
-    + replace (γ x0) with ((cons y (γ x) γ) x0) at 1.
-      2: { unfold cons. destruct (y == x0). done. done. }
-      eapply sem_var.
-  - pick fresh z and apply sem_abs.
-    spec z.
-    rewrite <- cons_cons; auto.
-    autorewrite with lngen in H1.
-    eapply H1. rewrite fv_tm_open_tm_wrt_tm_upper.  simpl. fsetdec.
+  unfold denot. simpl.
+  rewrite size_tm_open_tm_wrt_tm_var.
+  f_equal.
+  extensionality D.
+  name_binder x0 Frx0.
+  simpl_env. 
+  rewrite -> (rename_open_denot x0 x); eauto.
 Qed.
 
 
-Lemma sem_rename : forall x y γ M v w,
-    x `notin` fv_tm M -> 
-    y `notin` fv_tm M ->
-    sem (cons x w γ) (M ^ x) v ->
-    sem (cons y w γ) (M ^ y) v.
-Proof.
-  intros x y γ M v w Fr1 Fr2 h.
-  destruct (x == y). subst. auto.
-  rewrite (subst_tm_intro x); auto.
-  remember (cons x w γ) as δ.
-  replace (cons y w γ) with (cons y (δ x) δ).
-  eapply sem_subst with (x:=x) (y:=y).
-  rewrite fv_tm_open_tm_wrt_tm_upper.  simpl. fsetdec.
-Admitted.
-  
+Create HintDb denot.
+#[export] Hint Opaque denot : denot.
+#[export] Hint Rewrite denot_var_b denot_var denot_app denot_lit 
+  denot_add denot_tnil denot_tcons : denot.
+(* no hint for abs, must pick fresh first *)
 
-Lemma sem_abs_ex : forall γ x v w N,
-      x `notin` fv_tm N ->
-      sem (cons x v γ) (N ^ x) w -> 
-      sem γ (abs N) (v ↦ w).
+Lemma weaken_denot1 : forall t ρ ρ1 ρ2, 
+    fv_tm t [<=] dom (ρ1 ++ ρ2) ->
+    uniq (ρ1 ++ ρ ++ ρ2) ->
+    denot t (ρ1 ++ ρ2) = denot t (ρ1 ++ ρ ++ ρ2). 
+Proof.
+  intro t.
+  eapply tm_induction with (t := t).
+  1: move=>i. 
+  2: move=>x.
+  3: move=>t1 t2 IH1 IH2. 
+  4: move=> u IH.
+  8: move=> t1 t2 IH1 IH2.
+  all: intros ρ ρ1 ρ2 FV U.
+  all: simpl_env in FV; simpl in FV. 
+  all: autorewrite with denot.
+  all: try solve [reflexivity].
+  + (* var *) 
+    destruct_uniq.
+    move: (access_app_P ρ1 x) => [A1|A2].
+    rewrite A1. rewrite A1. auto.
+    move: (A2 ρ2) => [A21 A22].
+    rewrite A22.
+    move: (A2 (ρ ++ ρ2)) => [A31 A32].
+    rewrite A32.
+    rewrite access_app_fresh; auto.
+    intro h.
+    solve_uniq.
+  + (* app *)
+    f_equal.
+    eapply IH1; simpl_env; eauto.
+    fsetdec.
+    eapply IH2; simpl_env; eauto.
+    fsetdec.
+  + pick fresh x.
+    repeat rewrite (denot_abs x).
+    simpl_env; fsetdec.
+    simpl_env; fsetdec.
+    f_equal.
+    extensionality D.
+    rewrite <- app_assoc.
+    erewrite IH; simpl_env; eauto.
+    rewrite fv_tm_open_tm_wrt_tm_upper; simpl; eauto.
+    fsetdec.
+  + f_equal.
+    eapply IH1; simpl_env; eauto.
+    fsetdec.
+    eapply IH2; simpl_env; eauto.
+    fsetdec.
+Qed.
+
+Lemma weaken_denot : forall t ρ2 ρ,
+   fv_tm t [<=] dom ρ2 ->
+   uniq (ρ ++ ρ2) ->
+   denot t ρ2 = denot t (ρ ++ ρ2). 
 Proof.
   intros.
-  pick fresh z and apply sem_abs.
-  eapply sem_rename; eauto.
+  unfold denot.
+  eapply weaken_denot1 with (ρ1 := nil); simpl; auto.
 Qed.
 
+(* Scoping predicates *)
 
-Definition tm_Id : tm := abs (var_b 0).
-
-Lemma denot_Id : sem empty tm_Id (⊥ ↦ ⊥).
+Lemma subst_denot : forall t x u ρ1 ρ2, 
+    scoped t (ρ1 ++ x ~ (denot u ρ2) ++ ρ2) ->
+    scoped u ρ2 ->
+    denot t (ρ1 ++ x ~ (denot u ρ2) ++ ρ2) =
+    denot (t [x ~> u]) (ρ1 ++ ρ2).
 Proof.
-  pick fresh x and apply sem_abs.
-  cbn. 
-  replace ⊥ with ((cons x ⊥ empty) x) at 2.
-  eapply sem_var.
-  unfold cons. rewrite eq_dec_refl.
-  reflexivity.
+  intro t.
+  eapply tm_induction with (t := t);
+  [move=>i|move=>y|move=>t1 t2 IH1 IH2|move=> t' IH|move=>k| | | move=> t1 t2 IH1 IH2].
+  all: intros x u ρ1 ρ2 ST SU.
+  all: simpl. 
+  all: simpl_env. 
+  all: autorewrite with denot.
+  all: try solve [reflexivity].
+  + destruct (y == x) eqn:EQ. subst.
+    ++ have NI: x `notin` dom ρ1.
+       { inversion ST. destruct_uniq. auto. }
+       have D2: fv_tm u [<=] dom ρ2. 
+       { inversion SU. auto. }
+       have U2: uniq (ρ1 ++ ρ2). 
+       { inversion ST. solve_uniq. }
+       rewrite access_app_fresh; auto.       
+       rewrite access_eq_var.
+       apply weaken_denot; eauto.
+    ++ repeat rewrite denot_var.
+       destruct (access_app_P ρ1 y) as [h1 | h2].
+       repeat rewrite h1. auto.
+       move: (h2 ρ2) => [N1 ->]. 
+       move: (h2 (x ~ denot u ρ2 ++ ρ2)) => [N3 ->].
+       rewrite access_neq_var; auto.
+  + move: (scoped_app_inv1 _ _ _ _ ST) => S1.
+    move: (scoped_app_inv2 _ _ _ _ ST) => S2.
+    f_equal.
+    eapply IH1; eauto.
+    eapply IH2; eauto.
+  + have LCU: lc_tm u. inversion SU. auto.
+    pick fresh z.
+    specialize (IH z ltac:(auto) x u).
+    simpl. simpl_env.
+    repeat rewrite (denot_abs z).
+    simpl_env. fsetdec.
+    simpl_env. rewrite fv_tm_subst_tm_upper. fsetdec. 
+    f_equal.
+    extensionality D.
+    have FZ: z `notin` (dom (ρ1 ++ x ~ denot u ρ2 ++ ρ2) \u fv_tm t').
+    simpl_env. fsetdec.
+    move: (scoped_abs_inv _ z t' D _ FZ ST) => h.
+    rewrite <- app_assoc.
+    rewrite IH; auto.
+    rewrite subst_tm_open_tm_wrt_tm. eauto.
+    rewrite subst_neq_var. auto.
+    reflexivity.
+  + move: (scoped_tcons_inv1 _ _ _ _ ST) => S1.
+    move: (scoped_tcons_inv2 _ _ _ _ ST) => S2.
+    f_equal.
+    eapply IH1; eauto.
+    eapply IH2; eauto.
 Qed.
 
-Definition tm_Delta : tm := abs (app (var_b 0) (var_b 0)).
-
-Lemma denot_Delta : forall v w, sem empty tm_Delta (((v ↦ w) ⊔ v) ↦ w).
+Lemma subst_denot1 :
+  forall (t : tm) (x : atom) (u : tm) (ρ : Env (P Value)),
+    scoped t (x ~ denot u ρ ++ ρ) 
+    -> scoped u ρ 
+    -> denot t (x ~ denot u ρ ++ ρ) = denot (t [x ~> u]) ρ.
 Proof.
-  intros. unfold tm_Delta.
-  pick fresh x and apply sem_abs.
-  eapply sem_app.
-  3: { eapply app_beta. }
-  + cbn. eapply sem_sub. eapply sem_var.
-    unfold cons. rewrite eq_dec_refl.
-    instantiate (1:=v).
-    eauto.
-  + cbn. eapply sem_sub. eapply sem_var.
-    unfold cons. rewrite eq_dec_refl.
-    eauto.
-Qed. 
-
-(** Denotation **)
-
-Definition Denotation := Env -> Value -> Prop.
-
-Definition E (M : tm) : Denotation := fun γ v => sem γ M v.
-
-Definition den_eq (D1 : Denotation) (D2: Denotation) : Prop :=
-  forall γ v, D1 γ v <-> D2 γ v.
-
-#[global] Instance Eq_den : Equivalence den_eq.
-constructor.
-- split; auto.
-- unfold Symmetric. intros x y h. intros γ v. specialize (h γ v). tauto.
-- unfold Transitive. intros x y z h1 h2. intros γ v.
-  specialize (h1 γ v).
-  specialize (h2 γ v).
-  tauto.
-Defined.
-
-(* Environment strengthening *)
-
-Lemma sub_env : forall γ M v, 
-    sem γ M v 
-    -> forall δ, env_sub γ δ
-    -> sem δ M v.
-Proof.
-  induction 1; intros; eauto.
-  - pick fresh x and apply sem_abs.
-    spec x.
-    eapply H0.
-    unfold env_sub.
-    intros y.
-    unfold cons.
-    destruct (x == y). auto. auto.
-Qed.
-
-Lemma ext_le : forall x u1 u2 γ, 
-    u1 ⊑ u2 ->
-    env_sub (cons x u1 γ) (cons x u2 γ).
-Proof.
-  intros. unfold env_sub, cons.
-  intros y.
-  (destruct (x == y)). auto.
-  auto.
-Qed.
-
-Lemma up_env : forall γ M x u1 u2 v, 
-    sem (cons x u1 γ) M v ->
-    u1 ⊑ u2  ->
-    sem (cons x u2 γ) M v.
-Proof.
-  intros.
-  eapply sub_env; eauto using ext_le.
-Qed.
-
-(* ** Value Membership and Inclusion ** *)
-
-Fixpoint v_mem (u : Value) (v: Value) : Prop :=
-  match v with 
-  | ⊥ => u = ⊥
-  | v ↦ w => u = (v ↦ w)
-  | v ⊔ w => v_mem u v \/ v_mem u w
-  end.
-
-Infix "∈" := v_mem (at level 50).
-
-Definition v_inc v w := forall u, u ∈ v -> u ∈ w.
-
-Infix "⊆" := v_inc (at level 50).
-
-Lemma mem_sub : forall u v, u ∈ v -> u ⊑ v.
-Proof. intros. induction v; inversion H; eauto. Qed.
-
-Lemma union_inc : forall u v w, 
-    u ⊆ w -> v ⊆ w -> (u ⊔ v) ⊆ w.
-Proof.
-  unfold v_inc.
-  intros.
-  simpl in H1.
-  destruct H1. eauto. eauto.
-Qed.
-
-(* ⊔⊆-inv *)
-Lemma union_inc_inv : forall u v w, 
-    (u ⊔ v) ⊆ w -> u ⊆ w /\ v ⊆ w.
-Proof.    
-  intros u v w s. split.
-  intros x h1. eapply s. simpl. left. auto.
-  intros x h1. eapply s. simpl. right. auto.
-Qed.
-
-
-Lemma inc_sub : forall u v, u ⊆ v -> u ⊑ v.
-Proof. intros u v s.
-       induction u; eauto.
-       + eapply mem_sub.
-         eapply s.
-         reflexivity.
-       + apply union_inc_inv in s. 
-         move: s => [s1 s2].
-         eauto.
-Qed.
-
-(* ↦⊆→∈  *)
-Lemma fun_inc_mem : forall v w u, 
-    (v ↦ w) ⊆ u -> (v ↦ w) ∈ u.
-Proof. 
-  intros. eapply H. reflexivity.
-Qed.
-
-(** Function values **)
-
-Inductive Fn : Value -> Prop :=
-  fn : forall u v w, u = (v ↦ w) -> Fn u.
-
-Definition all_fns (v:Value) : Prop :=
-  forall u , u ∈ v -> Fn u.
-
-Lemma bot_not_Fn : ~ (Fn ⊥).
-Proof.
-  intros h. inversion h. done.
-Qed.
-
-Lemma all_fns_mem : forall u,
-    all_fns u -> exists v, exists w, (v ↦ w) ∈ u.
-Proof.
-  intros u f.
-  induction u; unfold all_fns in *.
-  - specialize (f ⊥ ltac:(reflexivity)).
-    apply bot_not_Fn in f. done.
-  - exists u1. exists u2. reflexivity.
-  - destruct IHu1 as [v [w h]].
-    + intros z h.
-      specialize (f z (or_introl h)). 
-      inversion f. done.
-    + exists v. exists w. simpl. auto.
-Qed.
-
-(** Domains and Codomains **)
-
-Fixpoint union_dom (u : Value) : Value :=
-  match u with 
-  | ⊥ => ⊥
-  | (v ↦ w) => v
-  | (u ⊔ u') => union_dom u ⊔ union_dom u'
-  end.
-
-
-Fixpoint union_cod (u : Value) : Value :=
-  match u with 
-  | ⊥ => ⊥
-  | (v ↦ w) => w
-  | (u ⊔ u') => union_cod u ⊔ union_cod u'
-  end.
-
-Lemma fn_in_union_dom : forall u v w, 
-    all_fns u 
-    -> (v↦ w) ∈ u
-    -> v ⊆ union_dom u.
-Proof.
-  intros u. 
-  induction u; intros v w fg hin u; inversion hin; subst; auto.
-  + intro uinv. simpl.
-    left.
-    eapply IHu1; eauto.
-    intros z hz. 
-    unfold all_fns in fg.
-    specialize (fg z (or_introl hz)).
-    inversion fg. done.
-  + intro uv. simpl.
-    right.
-    eapply IHu2; eauto.
-    intros z hz.
-    unfold all_fns in fg.
-    specialize (fg z (or_intror hz)).
-    inversion fg. done.
-Qed.
-
-Lemma sub_fn_union_cod : forall u v w, 
-     u ⊆ (v↦ w)
-    -> union_cod u ⊆ w.
-Proof.
-  intros u v w s; induction u; simpl in *.
-  + intros u' h; inversion h; subst.
-    specialize (s ⊥ ltac:(reflexivity)). inversion s.
-  + intros u' m. specialize (s (u1 ↦ u2) ltac:(reflexivity)).
-    inversion s. subst. auto.
-  + intros u' h; inversion h; subst.
-    ++ eapply IHu1; auto.  intros C z.  eapply s. simpl. left. auto.
-    ++ eapply IHu2; auto.  intros C z.  eapply s. simpl. right. auto.
-Qed.
-
-Definition factor := 
-  fun (u u' v w : Value) => 
-    (all_fns u') /\ (u' ⊆ u) /\ (union_dom u' ⊑ v) /\ (w ⊑ union_cod u').
-
-
-(* Inversion of less-than for functions, case for trans *)
-
-Lemma sub_inv_trans : forall u' u2 u, 
-    all_fns u' -> u' ⊆ u
-    -> (forall v' w', (v' ↦ w') ∈ u -> exists u3, factor u2 u3 v' w')
-    -> exists u3, factor u2 u3 (union_dom u') (union_cod u').
-Proof.
-intros u' u2 u fu' hsub IH.
-induction u'.
-- exfalso. apply bot_not_Fn. 
-  eapply fu'. reflexivity.  
-- apply IH.
-  eapply fun_inc_mem.
-  simpl. auto.
-- unfold all_fns in *. 
-  destruct (union_inc_inv _ _ _ hsub) as [h1' h2'].
-  destruct IHu'1 as [u31 [ fu21' [u31u2 [de1du1 cu1cu31]]]]. 2: { exact h1'. }
-  intros z h. specialize (fu' z (or_introl h)). inversion fu'. done.
-  destruct IHu'2 as [u32 [ fu22' [u32u2 [de1du2 cu1cu32]]]]. 2: { exact h2'. }
-  intros z h. specialize (fu' z (or_intror h)). inversion fu'. done.
-  exists (v_union u31 u32).
-  repeat split.
-  + unfold factor, all_fns in *.
-    intros v' x. inversion x. eapply fu21'. auto.
-    eapply fu22'. auto.
-  + eapply union_inc; eauto.
-  + simpl. eapply v_sub_mono; auto.
-  + simpl. eapply v_sub_mono; auto.
-Qed.
-
-(* Inversion of less-than for functions *)
-
-Lemma sub_inv : forall u1 u2, u1 ⊑ u2  
-                  -> forall v w, (v ↦ w) ∈ u1
-                  -> exists u3, factor u2 u3 v w.
-Proof.
-  intros u1 u2 h.
-  induction h. 
-  - intros v1 w1 h1. inversion h1.
-  - intros v1 w1 m.
-    inversion m; eauto. 
-  - intros v1 w1 m.
-    destruct (IHh _ _ m) as [u31 [fu31 [u31u21 [domu31v wcodu31]]]].
-    exists u31. repeat split.
-    + apply fu31.      
-    + intros C z. simpl. left. eauto.
-    + apply domu31v.
-    + apply wcodu31.
-  - intros v1 w1 m.
-    destruct (IHh _ _ m) as [u31 [fu31 [u31u21 [domu31v wcodu31]]]].
-    exists u31. repeat split.
-    + apply fu31.
-    + intros C z. simpl. right. eauto.
-    + apply domu31v.
-    + apply wcodu31.
-  - (* sub_trans *) 
-    intros v1 w1 m. 
-    edestruct (IHh1 _ _ m) as [ u' [ fu' [u'u [ domu'v wcodu']]]].
-    move: sub_inv_trans => f.
-    edestruct (sub_inv_trans _ _ _ fu' u'u IHh2)
-      as [ u3 [ fu3 [ u3u2 [ domu3domu' codu'codu3]]]]. 
-    exists u3.
-    repeat split.
-    + exact fu3.
-    + exact u3u2.
-    + eapply v_sub_trans. exact domu3domu'. exact domu'v.
-    + eapply v_sub_trans. exact wcodu'. exact codu'codu3.
-  - intros v1 w1 h.  inversion h. subst.
-    exists ( v' ↦ w' ). repeat split.
-    + unfold all_fns. intros. econstructor. eauto.
-    + unfold v_inc. tauto.
-    + simpl. auto.
-    + simpl. auto.
-  - intros. inversion H. subst.
-    exists ((v ↦ w) ⊔ (v ↦ w')).
-    repeat split.
-    + unfold all_fns. intros u h. inversion h. eapply fn. eauto.
-      eapply fn. eauto.
-    + intros y x. inversion x. eauto. eauto.
-    + eapply v_sub_conj_L. eapply v_sub_refl. eapply v_sub_refl.
-    + simpl. eapply v_sub_refl.
-Qed.
-
-Lemma sub_inv_fun : forall v w u1, 
-    (v ↦ w) ⊑ u1
-  -> exists u2, all_fns u2 /\ u2 ⊆ u1 /\
-            (forall v' w', (v' ↦ w') ∈ u2 -> v' ⊑ v) 
-          /\ w ⊑ union_cod u2.
-Proof.
-  intros v w u1 abc.
-  destruct (sub_inv _ _ abc v w) as [u2 [f [u2u1 [db cc]]]]; eauto.
-  unfold v_mem. auto.
-  exists u2. repeat split.
-  + exact f.
-  + exact u2u1.
-  + intros D E m. eapply v_sub_trans.
-    eapply inc_sub. eapply fn_in_union_dom. exact f. exact m. exact db.
-  + exact cc.
-Qed. 
-
-Lemma sub_fun_inv : forall v w v' w', 
-    (v ↦ w) ⊑ (v' ↦ w')
-    -> (v' ⊑ v) /\ w ⊑ w'.
-Proof.
-  intros v w v' w' lt.
-  destruct (sub_inv_fun _ _ _ lt) as [ Γ [ f [ Γv34 [ lt1 lt2 ]]]].
-  destruct (all_fns_mem _ f) as [ u [ u' uu'Γ]].
-  move: (Γv34 _ uu'Γ) => Eq.
-  inversion Eq. subst.
-  split.
-  + eapply lt1; eauto.
-  + eapply v_sub_trans. eapply lt2.
-    eapply inc_sub. eapply sub_fn_union_cod. eauto.
+  intros. 
+  eapply subst_denot with (ρ1 := nil); auto. 
 Qed.
