coq/Scoped.v
@@ -1,0 +1,114 @@
+(* ------------------------------------------------------------ *)
+(* Scoping                                                      *)
+(* ------------------------------------------------------------ *)
+
+Require Import Coq.Logic.FunctionalExtensionality.
+Require Import Coq.Classes.RelationClasses.
+Require Coq.Relations.Relation_Definitions.
+Require Import Lia.
+
+Require Export lc.tactics.
+Require Import lc.Env.
+
+Import LCNotations.
+Open Scope tm.
+
+Section Scoped.
+
+Variable A : Type.
+
+Inductive scoped t (ρ : Env A) :=
+  scoped_intro : 
+    fv_tm t [<=] dom ρ -> uniq ρ -> lc_tm t -> scoped t ρ.
+
+Lemma scoped_app : forall t1 t2 ρ,
+    scoped t1 ρ -> scoped t2 ρ -> 
+    scoped (app t1 t2) ρ.
+Proof.
+  intros. inversion H. inversion H0. econstructor; eauto.
+  simpl. fsetdec.
+Qed.
+
+Lemma scoped_app_inv1 : forall t1 t2 ρ,
+    scoped (app t1 t2) ρ ->
+    scoped t1 ρ.
+Proof.
+  intros. inversion H.
+  simpl in *. inversion H2.
+  econstructor; eauto. 
+  fsetdec.
+Qed.
+
+Lemma scoped_app_inv2 : forall t1 t2 ρ,
+    scoped (app t1 t2) ρ ->
+    scoped t2 ρ.
+Proof.
+  intros. inversion H.
+  simpl in *. inversion H2.
+  econstructor; eauto. 
+  fsetdec.
+Qed.
+
+
+Lemma scoped_tcons : forall t1 t2 ρ,
+    scoped t1 ρ -> scoped t2 ρ -> 
+    scoped (tcons t1 t2) ρ.
+Proof.
+  intros. inversion H. inversion H0. econstructor; eauto.
+  simpl. fsetdec.
+Qed.
+
+Lemma scoped_tcons_inv1 : forall t1 t2 ρ,
+    scoped (tcons t1 t2) ρ ->
+    scoped t1 ρ.
+Proof.
+  intros. inversion H.
+  simpl in *. inversion H2.
+  econstructor; eauto. 
+  fsetdec.
+Qed.
+
+Lemma scoped_tcons_inv2 : forall t1 t2 ρ,
+    scoped (tcons t1 t2) ρ ->
+    scoped t2 ρ.
+Proof.
+  intros. inversion H.
+  simpl in *. inversion H2.
+  econstructor; eauto. 
+  fsetdec.
+Qed.
+
+Lemma scoped_abs : forall x t1 D ρ, 
+  x `notin` dom ρ \u fv_tm t1
+  -> scoped (t1 ^ x) (x ~ D ++ ρ)
+  -> scoped (abs t1) ρ.
+Proof. 
+  intros. destruct H0.
+  simpl_env in s.
+  rewrite <- fv_tm_open_tm_wrt_tm_lower in s.
+  destruct_uniq.
+  constructor. simpl. fsetdec.
+  auto.
+  eapply (lc_abs_exists x).
+  auto.
+Qed.
+
+Lemma scoped_abs_inv : forall x t1 D ρ, 
+  x `notin` dom ρ \u fv_tm t1
+  -> scoped (abs t1) ρ
+  -> scoped (t1 ^ x) (x ~ D ++ ρ).
+Proof.
+  intros.
+  destruct H0. simpl in s. inversion l.
+  econstructor; eauto.
+  autorewrite with lngen.
+  simpl_env.
+  subst.
+  simpl. fsetdec.
+Qed.
+
+End Scoped.
+
+Arguments scoped {_}.
+
+#[export] Hint Constructors scoped : core.
