coq/congruence_theory.v
@@ -1,0 +1,188 @@
+(* Definitions over P Values respect ⊆ and ≃ *)
+
+Require Import Coq.Logic.FunctionalExtensionality.
+Require Import Coq.Classes.RelationClasses.
+Require Coq.Relations.Relation_Definitions.
+Require Import Lia.
+
+Require Export lc.tactics.
+Require Import lc.List.
+Require Import lc.Env.
+Require Import lc.SetsAsPredicates.
+Import SetNotations.
+Local Open Scope set_scope.
+
+Require Import lc.Container.
+Require Import lc.Scoped.
+
+(* Definitions *)
+Require Import lc.model_definitions.
+
+Require Import lc.denot.
+
+Require Import lc.valid_theory.
+
+Import EnvNotations.
+Import LCNotations.
+
+(*  Application is a Congruence ------------------------------------------------ *)
+
+Lemma CONS_mono_sub { D1 D2 D3 D4 } :
+    D1 ⊆ D3 -> D2 ⊆ D4 -> ((CONS D1 D2) ⊆ (CONS D3 D4)).
+Proof.  
+  intros D13 D24 w C. 
+  unfold CONS, In in C.
+  destruct w; simpl in C; try done.
+  destruct l; try done.
+  move: C => [ d1 d2 ].
+  unfold CONS, In. split.
+  eapply D13; auto.
+  eapply D24; auto.
+Qed.
+
+Lemma CONS_cong { D1 D2 D3 D4 } :
+    D1 ≃ D3 -> D2 ≃ D4 -> ((CONS D1 D2) ≃ (CONS D3 D4)).
+Proof.
+  intros [ d13 d31 ] [ d24 d42 ].
+  split; eapply CONS_mono_sub; eauto.
+Qed.
+
+#[export] Instance Proper_Included_CONS : Proper (Included ==> Included ==> Included) CONS. 
+unfold Proper. intros x1 y1 E1 x2 y2 E2. eapply CONS_mono_sub; eauto. Qed.
+
+#[export] Instance Proper_Same_CONS : Proper (Same_set ==> Same_set ==> Same_set) CONS. 
+unfold Proper. intros x1 y1 E1 x2 y2 E2. eapply CONS_cong; eauto. Qed.
+
+(*  Application is a Congruence ------------------------------------------------ *)
+                          
+
+Lemma APPLY_mono_sub { D1 D2 D3 D4 } :
+    D1 ⊆ D3 -> D2 ⊆ D4 -> ((D1 ▩ D2) ⊆ (D3 ▩ D4)).
+Proof.  
+  intros D13 D24 w APP. 
+  inversion APP; subst; unfold Included in *.
+  + apply FUNWRONG. eauto.
+  + apply ARGWRONG. eauto.
+  + apply BETA with (V:=V); eauto.
+    intros d z. eauto.
+  + apply PROJ with (VS := VS) (k := k); eauto.
+Qed.
+
+Lemma APPLY_cong { D1 D2 D3 D4 } :
+    D1 ≃ D3 -> D2 ≃ D4 -> ((D1 ▩ D2) ≃ (D3 ▩ D4)).
+Proof.
+  intros [ d13 d31 ] [ d24 d42 ].
+  split; eapply APPLY_mono_sub; eauto.
+Qed.
+
+#[export] Instance Proper_Included_APPLY : Proper (Included ==> Included ==> Included) APPLY. 
+unfold Proper. intros x1 y1 E1 x2 y2 E2. eapply APPLY_mono_sub; eauto. Qed.
+
+#[export] Instance Proper_Same_APPLY : Proper (Same_set ==> Same_set ==> Same_set) APPLY. 
+unfold Proper. intros x1 y1 E1 x2 y2 E2. eapply APPLY_cong; eauto. Qed.
+
+
+(*  Abstraction is Extensional ---- -------------------------------------- *)
+
+(* Λ-ext-⊆  *)
+
+(* NOTE: By restricting the hypothesis to only valid sets, we strengthen 
+   the result. But this depends on the definition of Λ which quantifies
+   over valid sets (i.e. CBV) *)
+Lemma Λ_ext_sub {F1 F2} :
+  (forall {X : P Value}, valid X -> F1 X ⊆ F2 X) -> Λ F1 ⊆ Λ F2.
+Proof.
+  intros F1F2 v Iv. destruct v eqn:E; inversion Iv; auto.
+  - split; auto. 
+    eapply F1F2; eauto. 
+Qed.
+
+Lemma Λ_ext {F1 F2} :
+  (forall {X}, valid X -> F1 X ≃ F2 X) -> Λ F1 ≃ Λ F2.
+Proof. 
+  intros g. split;
+  eapply Λ_ext_sub; intros X NEX; destruct (g X); eauto.
+Qed.
+
+(* ---------------------------------------------------- *)
+
+(* Sub environments ⊆e *)
+
+Lemma Reflexive_sub_env {ρ:Env (P Value)} : uniq ρ -> ρ ⊆e ρ.
+Proof.
+  intros. eapply Env.Forall2_refl; eauto.
+  typeclasses eauto.
+Qed.
+
+#[export] Hint Resolve Reflexive_sub_env : core.
+
+#[export] Instance Transitive_sub_env : 
+  Transitive (@Env.Forall2 (P Value) (P Value) Included).
+Proof. typeclasses eauto. Qed.
+
+Lemma extend_sub_env {ρ ρ': Env (P Value)}{y X} :
+  y `notin` dom ρ ->
+  ρ ⊆e ρ' -> (y ~ X ++ ρ) ⊆e (y ~ X ++ ρ' ).
+Proof. intros; econstructor; eauto. reflexivity. Qed.
+
+#[export] Hint Resolve extend_sub_env : core.
+
+(* ---------------------------------------------------- *)
+
+(* Why can we not get rid of this???? *)
+Ltac gather_atoms ::=
+  let A := gather_atoms_with (fun x : vars => x) in
+  let B := gather_atoms_with (fun x : var => {{ x }}) in
+  let C := gather_atoms_with (fun x => fv_tm x) in
+  let D := gather_atoms_with (fun x : list (atom * P Value) => dom x) in
+  let E := gather_atoms_with (fun x : Rho => dom x) in
+  constr:(A \u B \u C \u D \u E).
+
+
+(* The denotation respects ≃ *)
+#[export] Instance Proper_denot : Proper (eq ==> same_env ==> Same_set) denot.
+Proof.
+  intros t1 t ->.
+  eapply tm_induction with (t := t);
+  [move=>i|move=>x|move=>t1 t2 IH1 IH2|move=> t' IH|move=>k| | | move=> t1 t2 IH1 IH2].
+  all: move => ρ1 ρ2 EQ.
+  all: autorewrite with denot.
+  all: try solve [reflexivity].
+  all: eauto using APPLY_cong, CONS_cong.
+  - destruct (FSetDecideAuxiliary.dec_In  x (dom ρ1)).
+    + apply Forall2_access with (f := Same_set); auto.
+    + rewrite access_fresh. auto.
+      rewrite access_fresh. erewrite Forall2_dom in H; eauto.
+      reflexivity.
+  - pick fresh x. 
+    repeat rewrite (denot_abs x). fsetdec. fsetdec.
+    eapply Λ_ext.
+    intros X neX.
+    eapply IH; eauto.
+    econstructor; eauto. 
+    reflexivity. 
+Qed.
+
+(* The denotation respects ⊆ *)
+#[export] Instance Proper_sub_denot : Proper (eq ==> Env.Forall2 Included ==> Included) denot.
+Proof.
+  intros t1 t ->.
+  eapply tm_induction with (t := t);
+  [move=>i|move=>x|move=>t1 t2 IH1 IH2|move=> t' IH|move=>k| | | move=> t1 t2 IH1 IH2].
+  all: move => ρ1 ρ2 SUB.
+  all: autorewrite with denot.
+  all: try solve [reflexivity].
+  all: eauto using APPLY_mono_sub, CONS_mono_sub.
+  - destruct (FSetDecideAuxiliary.dec_In  x (dom ρ1)).
+    + apply Forall2_access with (f := Included); auto.
+    + rewrite access_fresh. auto.
+      rewrite access_fresh. erewrite Forall2_dom in H; eauto.
+      reflexivity.
+  - pick fresh x. 
+    repeat rewrite(denot_abs x). fsetdec. fsetdec.
+    eapply Λ_ext_sub.
+    intros X neX.
+    eapply IH. fsetdec.
+    econstructor; eauto.
+    reflexivity.
+Qed.
