coq/model_definitions.v
@@ -1,0 +1,278 @@
+Require Import Coq.Logic.FunctionalExtensionality.
+Require Import Coq.Classes.RelationClasses.
+Require Coq.Relations.Relation_Definitions.
+Require Import Lia.
+
+Require Export lc.tactics.
+Require Import lc.List.
+Require Import lc.Env.
+Require Import lc.Container.
+
+Require Import lc.Monad.
+Import MonadNotation.
+Open Scope monad_scope.
+
+Require Import lc.SetsAsPredicates.
+Import SetNotations.
+Local Open Scope set_scope.
+
+
+Inductive Value : Type :=
+  (* natural number *)
+  | v_nat : nat -> Value
+
+  (* one entry in a function's table *)
+  | v_map : list Value -> Value -> Value
+
+  (* trivial function value, evaluated to a value but never applied *)
+  | v_fun : Value
+
+  (* list/tuple of values *)
+  | v_list : list Value -> Value
+
+  (* dynamic type error *)
+  | v_wrong : Value
+.
+
+#[export] Hint Constructors Value : core.
+
+Infix "↦" := v_map (at level 85, right associativity).
+
+
+(* ------------ Valid or "succeeds" ------------------ *)
+
+Definition valid (V : P Value) : Type :=
+  nonemptyT V * not (v_wrong ∈ V).
+
+Definition valid_mem (V : list Value) : Prop :=
+  V <> nil /\ not (List.In v_wrong V).
+
+(* ------------ Semantic Operators ------------------ *)
+
+Definition NAT : nat -> P Value :=
+  fun j v => match v with 
+          | v_nat k => j = k
+          | _ => False
+          end.
+
+Definition LIST : list (P Value) -> P Value  :=
+  fun DS w => 
+    match w with 
+    | v_list WS => Forall2 Ensembles.In DS WS
+    | _ => False
+    end.
+
+Definition NIL : P Value := ⌈ v_list nil ⌉.
+
+Definition CONS : P Value -> P Value -> P Value := 
+  fun V W x => 
+    match x with 
+    | v_list (v :: w) => (v ∈ V) /\ (v_list w ∈ W)
+    | _ => False
+    end.
+
+Definition Λ : (P Value -> P Value) -> P Value :=
+  fun f => fun v => match v with 
+          | (V ↦ w) => (w ∈ f (mem V)) /\ valid_mem V  (* CBV *)
+          | v_fun => True
+          | _ => False
+          end.
+
+(* It is a little easier to specify this as an inductive relation 
+   than as a function. The cases don't overlap, but we don't need
+   to know that at definition time.
+*)
+
+Inductive APPLY : P Value -> P Value -> Value -> Prop :=
+  | FUNWRONG : forall D1 D2,
+     (v_wrong ∈ D1) ->
+     APPLY D1 D2 v_wrong
+  | ARGWRONG : forall D1 D2,
+     (v_wrong ∈ D2) 
+     -> APPLY D1 D2 v_wrong
+  | BETA : forall D1 D2 w V,
+     (V ↦ w ∈ D1) -> (mem V ⊆ D2) -> valid_mem V ->
+     APPLY D1 D2 w
+  | PROJ   : forall D1 D2 w VS k, 
+     (v_list VS ∈ D1) -> (v_nat k ∈ D2) -> nth_error VS k = Some w
+     -> APPLY D1 D2 w.
+(* ADD these two for more wrong *)
+(*
+  | FUNWRONG2 : forall D1 D2 x,
+     x ∈ D1 -> (Inconsistent x v_fun /\ forall XS, Inconsistent x (v_list XS)) ->
+     APPLY D1 D2 v_wrong
+  | ARGWRONG2 : forall D1 D2 VS x, 
+     (v_list VS ∈ D1) -> 
+     (x ∈ D2) -> 
+     (forall k, Inconsistent x (v_nat k)) ->
+     APPLY D1 D2 v_wrong. *)
+
+Infix "▩" := APPLY (at level 90).
+
+
+#[export] Hint Constructors APPLY : core.
+
+Definition ADD : P Value :=
+  fun w => 
+    match w with 
+    | (V ↦ v_nat k) => 
+        exists i j, ((v_list (v_nat i :: v_nat j :: nil)) ∈ mem V) /\ k = i + j
+    | V ↦ v_wrong => 
+        not (exists i j, v_list (v_nat i :: v_nat j :: nil) ∈ mem V)
+    | _ => False
+    end.
+
+(* ------------------------------------------------------- *)
+
+Definition finite (X : P Value) : Prop := 
+  exists E, (X ≃ mem E) /\ E <> nil.
+
+Definition continuous (F : P Value -> P Value) : Set :=
+  forall X E, mem E ⊆ F X -> valid X 
+         -> exists D, (mem D ⊆ X) /\ ((mem E) ⊆ F (mem D)) /\ valid_mem D.
+
+Definition monotone (F : P Value -> P Value) : Set := 
+  forall D1 D2, (D1 ⊆ D2) -> F D1 ⊆ F D2.
+
+(* ------------------------------------------------------- *)
+
+Definition Rho := Env (P Value).
+
+Ltac gather_atoms ::=
+  let A := gather_atoms_with (fun x : vars => x) in
+  let B := gather_atoms_with (fun x : var => {{ x }}) in
+  let C := gather_atoms_with (fun x => fv_tm x) in
+  let D := gather_atoms_with (fun x : list (atom * P Value) => dom x) in
+  let E := gather_atoms_with (fun x : Rho => dom x) in
+  constr:(A \u B \u C \u D \u E).
+
+Module EnvNotations.
+Notation "ρ ⋅ x" := (access ⌈ v_wrong ⌉ ρ x) (at level 50).
+Infix "⊔e" := (map2 Union) (at level 60).
+Infix "⊆e" := (Env.Forall2 Included) (at level 50).
+End EnvNotations.
+Import EnvNotations.
+
+Definition nonempty_env : Rho -> Type := Env.ForallT nonemptyT.
+
+Definition valid_env : Rho -> Type := Env.ForallT valid. 
+
+Definition finite_env : Rho -> Type := Env.ForallT finite.
+
+Definition monotone_env (D : Rho -> P Value) := 
+  forall ρ ρ' , ρ ⊆e ρ' -> (D ρ) ⊆ D ρ'.
+
+Definition continuous_In (D:Rho -> P Value) (ρ:Rho) (v:Value) : Prop :=
+  v ∈ D ρ -> exists ρ' , exists (pf : finite_env ρ'),  ρ' ⊆e ρ /\ (v ∈ D ρ').
+
+Definition continuous_env (D:Rho -> P Value) (ρ:Rho) : Prop :=
+  forall v, continuous_In D ρ v.
+
+(* ------------------------------------------------------- *)
+
+Definition sub_env : Rho -> Rho -> Prop := Env.Forall2 Included.
+
+Definition same_env : Rho -> Rho -> Prop := Env.Forall2 Same_set.
+
+(* ------------------------------------------------------- *)
+
+Import LCNotations.
+Open Scope tm.
+
+(* Denotation function *)
+(* `n` is is a termination metric. *)
+Fixpoint denot_n (n : nat) (a : tm) (ρ : Rho) : P Value :=
+  match n with
+  | O => fun _ => False
+  | S m => 
+     match a with 
+     | var_b _ => ⌈ v_wrong ⌉
+     | var_f x => ρ ⋅ x 
+     | app t u   => 
+         denot_n m t ρ ▩ denot_n m u ρ
+     | abs t => 
+         let x := fresh_for (dom ρ \u fv_tm t) in 
+         Λ (fun D => denot_n m (t ^ x) (x ~ D ++ ρ))
+     | lit k => NAT k
+     | add => ADD
+     | tnil => NIL
+     | tcons t u => CONS (denot_n m t ρ) (denot_n m u ρ)
+     end
+  end.
+
+
+(* ------------------------------------------------- *)
+
+(* Consistent values: we model function values as a set of approximations
+
+   But now that we have different sorts of values, those approximations should
+   all agree with eachother.
+
+   We can define this concept by first identifying the head of a value. 
+   Two values will *definitely* be inconsistent if they have different heads.
+   But they could have the same head if inside the value
+
+*)
+
+Inductive v_head := 
+   h_nat  : nat -> v_head 
+  | h_fun  : v_head
+  | h_list : v_head
+  | h_wrong : v_head 
+.
+
+Definition head (v : Value) : v_head := 
+  match v with 
+  | v_nat k => h_nat k
+  | v_map _ _ => h_fun
+  | v_fun => h_fun
+  | v_list _ => h_list
+  | v_wrong => h_wrong
+  end.
+
+
+Inductive Consistent : Value -> Value -> Prop :=
+  | c_nat : forall i, Consistent (v_nat i) (v_nat i)
+  | c_list : forall XS YS, Forall2 Consistent XS YS ->  Consistent (v_list XS) (v_list YS)
+  | c_wrong : Consistent v_wrong v_wrong
+
+  | c_fun : Consistent v_fun v_fun
+  | c_fun1 : forall X r, Consistent v_fun (X ↦ r)
+  | c_fun2 : forall X r, Consistent (X ↦ r) v_fun
+
+  | c_map2 : forall X1 X2 r1 r2, 
+      Consistent r1 r2 -> 
+      Consistent (X1 ↦ r1) (X2 ↦ r2)
+  | c_map1 : forall X1 X2 r1 r2, 
+      Exists2_any Inconsistent X1 X2 ->
+      Consistent (X1 ↦ r1) (X2 ↦ r2)
+
+with Inconsistent : Value -> Value -> Prop :=
+  | i_head : forall x y, 
+      head x <> head y ->
+      Inconsistent x y
+  | i_list_l : forall XS YS, 
+      length XS <> length YS ->
+      Inconsistent (v_list XS) (v_list YS)      
+  | i_list_e : forall XS YS,
+      Exists2 Inconsistent XS YS ->
+      Inconsistent (v_list XS) (v_list YS)
+  | i_map : forall X1 X2 r1 r2,
+      Forall2_any Consistent X1 X2 ->
+      Inconsistent r1 r2 ->
+      Inconsistent (X1 ↦ r1) (X2 ↦ r2).
+
+#[export] Hint Constructors Consistent Inconsistent v_head : core.
+
+
+(* Two sets are consistent if all of their elements 
+   are consistent. *)
+Definition ConsistentSets V1 V2 := 
+    forall x y, x ∈ V1 -> y ∈ V2 -> Consistent x y.
+
+Definition ConsistentSet V := ConsistentSets V V.
+
+Definition consistent_env : Rho -> Type := Env.ForallT ConsistentSet. 
+
+(* ------------------------------------------------------------------------------- *)
+
