coq/valid_theory.v
@@ -1,0 +1,141 @@
+Require Import Coq.Logic.FunctionalExtensionality.
+Require Import Coq.Classes.RelationClasses.
+Require Coq.Relations.Relation_Definitions.
+Require Import Lia.
+
+Require Export lc.tactics.
+Require Import lc.List.
+Require Import lc.Env.
+Require Import lc.SetsAsPredicates.
+Import SetNotations.
+Local Open Scope set_scope.
+Require Import lc.Monad.
+Import MonadNotation.
+Open Scope monad_scope.
+Require Import lc.Container.
+Require Import lc.Scoped.
+
+(* Definitions *)
+Require Import lc.model_definitions.
+
+Import EnvNotations.
+Import LCNotations.
+
+Lemma valid_mem_valid {V} : valid_mem V -> valid (mem V).
+Proof.
+  intros [V1 V2].
+  destruct V; simpl in *. done.
+  split. exists v. auto. eauto.
+Qed.
+
+
+(* valid sets are inhabited *)
+Definition valid_is_nonempty V : valid V -> nonemptyT V := fst.
+
+Lemma valid_nonempty_mem : forall V, 
+      valid_mem V -> nonemptyT (mem V).
+Proof. intros. eapply valid_is_nonempty.
+       eapply valid_mem_valid; auto. Qed.
+
+(* And do not contain wrong *)
+Lemma valid_not_wrong {X} : valid X -> not (v_wrong ∈ X).
+Proof. intros [x h1]; done. Qed.
+
+Lemma valid_mem_nonnil {V} : valid_mem V -> V <> nil.
+Proof. intros [h _]; auto. Qed.
+
+Lemma valid_mem_not_wrong {V} : valid_mem V -> not (List.In v_wrong V).
+Proof. intros [h j]; auto. Qed.
+
+
+(* A finite, inhabited subset of a valid set is valid *)
+Lemma valid_sub_valid_mem {D a} :
+  D <> nil -> valid a -> mem D ⊆ a -> valid_mem D.
+Proof.
+  intros NE [V1 V2] S.
+  inversion V1.
+  split; auto.
+Qed.
+
+#[export] Hint Immediate valid_is_nonempty valid_nonempty_mem valid_not_wrong valid_mem_valid valid_mem_nonnil valid_mem_not_wrong valid_sub_valid_mem : core.
+
+Lemma valid_join : forall v1 v2, 
+    valid v1 -> 
+    valid v2 ->
+    valid (v1 ∪ v2).
+Proof.
+  intros v1 v2 [[x1 I1] h1] [[x2 I2] h2].
+  split. 
+  exists x1. eapply Union_introl; eauto.
+  intro h. inversion h; subst; done.
+Qed.
+
+
+(* valid operators *)
+
+Lemma valid_NIL : valid NIL.
+Proof.
+  unfold NIL, valid.
+  split. econstructor; eauto. intro h; inversion h.
+Qed.
+
+Lemma valid_CONS {x y z} : valid x -> valid y -> v_list z ∈ y -> valid (CONS x y).
+Proof.
+  intros [[vx h1] nx] [[vl h2] nl] In. unfold CONS.
+  split.
+  - exists (v_list (vx :: z)). cbv. eauto.
+  - intro h. inversion h.
+Qed. 
+
+Lemma valid_NAT : forall k, valid (NAT k).
+Proof.
+  intros k. unfold NAT, valid. split.
+  exists (v_nat k); eauto. cbn. auto.
+  intro h; inversion h.
+Qed.
+
+Lemma valid_ADD : valid ADD.
+Proof. 
+  unfold ADD, valid.
+  split.
+  exists ( (v_list (v_nat 0 :: v_nat 0 :: nil) :: nil) ↦ v_nat 0). 
+  cbn.
+  exists 0. exists 0. split.  auto. auto.
+  intro h. inversion h.
+Qed.
+
+Lemma valid_Λ : forall F, valid (Λ F).
+Proof. 
+  intros F. 
+  split. cbv.
+  exists v_fun. auto. 
+  unfold In. done.
+Qed.
+
+ 
+Lemma valid_LIST : forall D, ForallT valid D -> valid (LIST D).
+induction 1. 
+split; auto.
+exists (v_list nil); done. 
+destruct IHX as [[xs nin] h].
+destruct p as [[y niny] hy]. 
+destruct xs; try done.
+split. 
+exists (v_list (y :: l0)). econstructor; eauto.
+eauto.
+Qed.
+
+(* Valid environments *)
+
+Lemma valid_nil : valid_env nil.
+Proof. unfold valid_env. eauto. Qed.
+
+#[export] Hint Resolve valid_nil : core.
+
+Lemma extend_valid_env {ρ x X} : 
+  x `notin` dom ρ ->
+  valid X -> 
+  valid_env ρ -> valid_env (x ~ X ++ ρ).
+Proof. intros Fr NEP NEX.  eapply ForallT_cons; eauto. Qed.
+
+#[export] Hint Resolve extend_valid_env : core.
