coq/value_theory.v
@@ -1,0 +1,367 @@
+Require Import Coq.Logic.FunctionalExtensionality.
+Require Import Coq.Classes.RelationClasses.
+Require Coq.Relations.Relation_Definitions.
+Require Import Lia.
+
+Require Export lc.tactics.
+Require Import lc.List.
+
+Require Import lc.SetsAsPredicates.
+Import SetNotations.
+Local Open Scope set_scope.
+
+
+Require Import lc.model_definitions.
+Require Import lc.denot.
+Require Import lc.valid_theory.
+
+
+(* 
+   The default induction principle for values is not
+   strong enough for lists in the v_map and v_list case. So we prove a stronger
+   version below.
+
+   Value_ind
+     : forall P : Value -> Prop,
+       (forall n : nat, P (v_nat n)) ->
+       (forall (l : list Value) (v : Value), P v -> P (v_map l v)) ->
+       P v_fun -> 
+       (forall l : list Value, P (v_list l)) -> 
+       P v_wrong -> 
+       forall v : Value, P v 
+*)
+
+Fixpoint Value_ind' (P : Value -> Prop)
+       (n : forall n : nat, P (v_nat n)) 
+       (m : forall (l : list Value) (v : Value), Forall P l -> P v -> P (v_map l v)) 
+       (f : P v_fun)
+       (l : (forall l : list Value, Forall P l -> P (v_list l)))
+       (w : P v_wrong) 
+       (v : Value) : P v := 
+  let rec := Value_ind' P n m f l w 
+  in
+  let fix rec_list (vs : list Value) : Forall P vs :=
+    match vs with 
+    | nil => Forall_nil _
+    | cons w ws => @Forall_cons Value P w ws (rec w) (rec_list ws)
+    end
+  in 
+  match v with 
+  | v_nat k => n k
+  | v_map X v => 
+      m X v (rec_list X) (rec v)
+  | v_fun => f
+  | v_list X => l X (rec_list X)
+  | v_wrong => w 
+  end.
+
+(* We do the same thing for Value_rect *)
+
+Fixpoint Value_rec' (P : Value -> Type)
+       (n : forall n : nat, P (v_nat n)) 
+       (m : forall (l : list Value) (v : Value),
+           ForallT P l -> P v -> P (v_map l v)) 
+       (f : P v_fun)
+       (l : (forall l : list Value, ForallT P l -> P (v_list l)))
+       (w : P v_wrong) (v : Value) : P v := 
+  let rec := Value_rec' P n m f l w 
+  in
+  let fix rec_list (vs : list Value) : ForallT P vs :=
+    match vs with 
+    | nil => ForallT_nil _
+    | cons w ws => @ForallT_cons Value P w ws (rec w) (rec_list ws)
+    end
+  in 
+  match v with 
+  | v_nat k => n k
+  | v_map X v => 
+      m X v (rec_list X) (rec v)
+  | v_fun => f
+  | v_list X => l X (rec_list X)
+  | v_wrong => w 
+  end.
+
+
+(* ----------------------------------------------- *)
+
+
+Definition ConsistentPointwiseList XS YS := 
+  Forall2 Consistent XS YS.
+Definition InconsistentPointwiseList XS YS := 
+  length XS <> length YS \/ Exists2 Inconsistent XS YS.
+Definition ConsistentAnyList XS YS := 
+  forall x y, List.In x XS -> List.In y YS -> Consistent x y.
+Definition InconsistentAnyList XS YS := 
+  (exists x y, List.In x XS /\ List.In y YS /\ Inconsistent x y).
+
+
+
+(* Two values cannot be both consistent and inconsistent. *)
+
+Lemma Consistent_Inconsistent_disjoint : 
+  forall x y, Consistent x y -> Inconsistent x y -> False.
+Proof.
+  intros x.
+  eapply Value_ind' with (P := fun x => 
+  forall y : Value, Consistent x y -> Inconsistent x y -> False).
+  all: intros.
+  all: try solve [inversion H; inversion H0; subst; done].
+  + inversion H2; inversion H1; subst.
+    all: try simpl in H3; try done.
+    - inversion H9; subst. clear H9.
+      eapply H0; eauto.
+    - inversion H9; subst. clear H9.
+    destruct H11 as [x1 [x2 [I1 [I2 ii]]]].
+    specialize (H5 _ _ I1 I2).
+    rewrite Forall_forall in H.
+    eapply H; eauto.
+  + inversion H0; inversion H1; subst. simpl in H5; try done.
+    - inversion H7; subst. eauto using Forall2_length.
+    - inversion H7; subst; clear H7.
+      clear H1 H0. move: YS H3 H6.
+      induction H; intros YS h1 h2;
+        inversion h1; inversion h2; subst.  
+      inversion H7; subst. eauto.
+      inversion H7; subst. eauto.
+Qed.
+
+(* Determining whether two values are consistent or inconsistent 
+   is decidable *)
+
+Definition ConsistentDecidable := fun v1 => forall v2 : Value, 
+                     {Consistent v1 v2} + {Inconsistent v1 v2}.
+
+
+
+Lemma dec_any : forall XS, ForallT ConsistentDecidable XS -> forall YS, { ConsistentAnyList XS YS } + {InconsistentAnyList XS YS}.
+induction XS.
+- intros h. intros ys. left. intros x y h1 h2. inversion h1.
+- intros h. inversion h. subst. clear h.
+  intros YS. unfold ConsistentDecidable in H1.
+  destruct (IHXS H2 YS).
+  + induction YS. left. intros x y h1 h2. inversion h2.
+    have CE: (ConsistentAnyList XS YS).
+    intros x y h1 h2. 
+    eapply c; eauto. simpl. eauto.
+    specialize (IHYS CE). destruct IHYS.
+    ++ destruct (H1 a0).       
+       left. 
+       { intros x y h1 h2.
+         destruct h1 as [EQ|INXS]; destruct h2 as [EQ2|INYS]; subst.
+         -- auto.
+         -- apply c0; eauto. simpl; auto.
+         -- apply c; eauto. simpl; auto.
+         -- apply CE; eauto.
+       } 
+       right. exists a . exists a0. simpl. split; auto.
+    ++ right. destruct i as [x [y [h1 [h2 h3]]]].
+       exists x. exists y. simpl. eauto.
+
+  + right. destruct i as [x1 [x2 [h1 [h2]]]].
+    exists x1. exists x2. simpl. split; eauto. 
+Qed.
+
+Lemma dec_point : forall XS,  ForallT ConsistentDecidable XS -> forall YS, { ConsistentPointwiseList XS YS } + {InconsistentPointwiseList XS YS}.
+Proof.  
+induction XS; intros IH [|y YS].
++ left. unfold ConsistentPointwiseList. eauto.
++ right. unfold InconsistentPointwiseList. simpl; left; auto.
++ right. left; simpl; auto.
++ inversion IH; subst. 
+  destruct (H1 y); destruct (IHXS H2 YS); unfold ConsistentPointwiseList in *; 
+    unfold InconsistentPointwiseList in *.
+  all: try solve [simpl; left; eauto].
+  all: try solve [right; destruct i; simpl; right; eauto].
+  right; destruct i; simpl.
+  left; eauto. 
+  right; eauto.
+Qed.  
+  
+Lemma dec_con : forall v1 v2, {Consistent v1 v2 } + {Inconsistent v1 v2 }.
+intros v1. 
+eapply Value_rec' with 
+(P := fun v1 =>  forall v2 : Value, {Consistent v1 v2} + {Inconsistent v1 v2}).
+all: intros.
+all: destruct v2.
+all: try solve [right; eapply i_head; simpl; done].
+all: try solve [left; eauto].
++ destruct (Nat.eq_dec n n0). subst.
+  left. eauto. right. eapply i_head; simpl. intro h.
+  inversion h. subst.  done.
++ destruct (H0 v2).
+  left. eapply c_map2; eauto.
+  destruct (dec_any l H l0).
+  right. eapply i_map; eauto.
+  left. eauto.
++ destruct (dec_point l H l0).
+  left; eauto.
+  right. destruct i; eauto.
+Qed.
+
+Lemma DecSetList : forall XS, ForallT ConsistentDecidable XS.
+intros XS. induction XS. econstructor; eauto.
+econstructor; eauto. unfold ConsistentDecidable. eapply dec_con; eauto.
+Qed.
+
+
+(* Consistency is also reflexive *)
+
+Definition ConsistentReflexive (x : Value) := Consistent x x.
+
+Lemma ConsistentPointwiseList_refl : forall XS, ForallT ConsistentReflexive XS -> ConsistentPointwiseList XS XS. 
+Proof.
+  induction 1; unfold ConsistentPointwiseList; eauto.
+Qed.
+
+#[export] Instance Consistent_refl : Reflexive Consistent.
+intro x.
+eapply Value_ind' with (P := ConsistentReflexive).
+all: unfold ConsistentReflexive; intros; eauto using ConsistentPointwiseList_refl.
+econstructor. rewrite <- Forall_Forall2. auto.
+Qed.
+
+
+(* ------------------------------------------------- *)
+(* Consistent sets *)
+
+Lemma ConsistentSets_sub {X1 X2 Y1 Y2} : 
+  ConsistentSets Y1 Y2 -> X1 ⊆ Y1 -> X2 ⊆ Y2 -> ConsistentSets X1 X2.
+Proof.
+  unfold ConsistentSets in *.
+  unfold Included in *. eauto.
+Qed.
+
+Lemma ConsistentSet_sub {X Y} : ConsistentSet Y -> X ⊆ Y -> ConsistentSet X.
+Proof.
+  unfold ConsistentSet, ConsistentSets in *.
+  unfold Included in *. eauto.
+Qed.
+
+(* Not transitive. The middle set may be empty! *)
+(* Instance ConsistentSets_Transitive : Transitive ConsistentSets. *)
+
+
+(* ------------------------------------------------- *)
+
+Definition APPLY_ConsistentSets : forall w1 w2 w1' w2', 
+    ConsistentSets w1 w1' -> 
+    ConsistentSets w2 w2' -> 
+    ConsistentSets (APPLY w1 w2) (APPLY w1' w2'). 
+Proof.
+  intros w1 w2 w1' w2' C1 C2.
+  unfold ConsistentSets in *.
+  intros x y h1 h2.
+
+  inversion h1; inversion h2; subst; eauto; clear h1 h2.
+  all: try (move: (C1 _ _ H H3) => h; inversion h; subst; auto).
+  all: try (move: (C1 _ _ H H5) => h; inversion h; subst; auto).
+  all: try (move: (C2 _ _ H H4) => h; inversion h; subst; auto).
+  all: try (move: (C2 _ _ H0 H5) => h; inversion h; subst; auto).
+
+  (* Application of a function to "wrong". This case is impossible because
+     the map's domain is valid and all elements of w2 are consistent with wrong. *) 
+  move: H5 => [NE NW]. 
+  exfalso.
+  have L: forall y, y ∈ w2' -> Consistent v_wrong y.
+  { intros. eauto. }
+  destruct V; try done.
+  specialize (L v ltac:(eauto)). inversion L. subst; simpl in NW. auto.
+
+  move: H1 => [NE NW]. 
+  exfalso.
+  have L: forall y, y ∈ w2 -> Consistent y v_wrong.
+  { intros. eauto. }
+  destruct V; try done.
+  specialize (L v ltac:(eauto)). inversion L. subst; simpl in NW. auto.
+
+  move: H3 => [x1 [x2 [I1 [I2 ii]]]].
+  have h3 : x1 ∈ w2. eapply H0; eauto.
+  have h4 : x2 ∈ w2'. eapply H6; eauto.
+  move: (C2 x1 x2 h3 h4) => h5.
+  assert False. eapply Consistent_Inconsistent_disjoint; eauto. done.
+
+  move: (C2 _ _ H0 H6)=> c1. inversion c1; subst; clear c1; eauto. 
+  clear h H H0 H5 H6.
+  move: k0 H1 H7.
+  induction H4; intros k0; destruct k0; simpl;  try done.
+  + intros h1 h2; inversion h1; inversion h2; subst. auto.
+  + intros h1 h2. eauto.
+Qed.
+
+Definition APPLY_ConsistentSet : forall w1 w2, 
+    ConsistentSet w1 -> 
+    ConsistentSet w2 -> 
+    ConsistentSet (APPLY w1 w2). 
+Proof.
+  intros.  unfold ConsistentSet in *.
+  eapply APPLY_ConsistentSets; eauto.
+Qed.
+
+Ltac gather_atoms ::=
+  let A := gather_atoms_with (fun x : vars => x) in
+  let B := gather_atoms_with (fun x : var => {{ x }}) in
+  let C := gather_atoms_with (fun x => fv_tm x) in
+  let D := gather_atoms_with (fun x : list (atom * P Value) => dom x) in
+  let E := gather_atoms_with (fun x : Rho => dom x) in
+  constr:(A \u B \u C \u D \u E).
+
+
+Lemma Consistent_denot :
+  forall t ρ1 ρ2, Env.ForallT2 ConsistentSets ρ1 ρ2 -> valid_env ρ1 -> valid_env ρ2 ->
+             ConsistentSets (denot t ρ1) (denot t ρ2).
+Proof.
+  intro t.
+  eapply tm_induction with (t := t);
+  [move=>i|move=>x|move=>t1 t2 IH1 IH2|move=> t' IH|move=>k| | | move=> t1 t2 IH1 IH2].
+  all: intros ρ1 ρ2 CR VR1 VR2.
+  all: autorewrite with denot.
+  all: intros x1 x2 I1 I2.
+  all: try solve [inversion I1; inversion I2; eauto].
+
+  - (* var *) 
+    induction CR; simpl in I1, I2.
+    ++ inversion I1. inversion I2. subst. auto.
+    ++ destruct (x == x0) eqn:E; rewrite E in I1, I2. eapply f; eauto.
+       inversion VR1. inversion VR2. eauto.
+
+  - (* app *)
+    move: (IH1 ρ1 ρ2 ltac:(eauto) ltac:(eauto) ltac:(eauto)) => C1.
+    move: (IH2 ρ1 ρ2 ltac:(eauto) ltac:(eauto) ltac:(eauto)) => C2.
+
+    move: (APPLY_ConsistentSets _ _ _ _ C1 C2) => CA.
+
+    eapply (CA x1 x2 I1 I2).
+
+  - (* abs *)
+    pick fresh y.
+    rewrite (denot_abs y) in I1; eauto.
+    rewrite (denot_abs y) in I2; eauto.
+    destruct x1; unfold In, Λ in I1; try done;
+    destruct x2; unfold In, Λ in I2; try done.
+    move: I1 => [I1 [Vl Cl]].
+    move: I2 => [I2 [Vl0 Cl0]].
+    destruct (dec_any l (DecSetList l) l0).
+    destruct (dec_con x1 x2). eapply c_map2; eauto.
+    ++ (* Domains are consistent, ranges are not. Should be a contradiction. *)
+      have CS: ConsistentSets (mem l) (mem l0). admit.
+      have V1:  valid_env (y ~ mem l ++ ρ1). econstructor; eauto. admit.
+      have V2:  valid_env (y ~ mem l0 ++ ρ2). admit.
+      move: (IH y ltac:(auto)) => h. 
+      specialize (h (y ~ mem l ++ ρ1) (y ~ mem l0 ++ ρ2)). 
+      have k9: Env.ForallT2 ConsistentSets (y ~ mem l ++ ρ1) (y ~ mem l0 ++ ρ2).
+      econstructor; eauto.
+      specialize (h ltac:(eauto) ltac:(eauto) ltac:(eauto)).
+      move: (h x1 x2 I1 I2) => C12.
+      exfalso. eapply Consistent_Inconsistent_disjoint; eauto.
+    ++ unfold InconsistentAnyList in i. 
+       eapply c_map1; eauto.
+  - (* nat *)
+    unfold NAT in *. 
+    destruct x1; try done.
+    destruct x2; try done.
+    inversion I1; inversion I2; subst; eauto.
+  - (* ADD: need a lemma that ADD is consistent *) 
+    admit.
+  - (* CONS: need a lemma about CONS *)
+    admit.
+Admitted.
